Fix typeclass inference problems

theories/MaxOfTwoNumbers/Computed/AllLogits.v
@@ -2,21 +2,17 @@ From NeuralNetInterp.MaxOfTwoNumbers Require Import Model.
 From NeuralNetInterp.Torch Require Import Tensor.
 From NeuralNetInterp.Util Require Import Pointed ValueExtraction.
 
-Local Notation prea := (logits all_tokens) (only parsing).
-Local Notation prev := (PArray.concretize prea) (only parsing).
-Local Definition pre := prev.
-
 Set NativeCompute Timing.
 (*Set NativeCompute Profiling.*)
 (* expected: about 45 minutes in vm, about 19 minutes in native *)
-Time Local Definition all_tokens_logits_concrete_value := native_compute pre.
+Time Local Definition all_tokens_logits_concrete_value := native_compute logits_all_tokens_concrete.
 
 Time Definition all_tokens_logits_concrete : PArray.concrete_tensor _ _ := (*Eval native_compute in pre *)Eval hnf in extract all_tokens_logits_concrete_value.
-Time Definition all_tokens_logits_concrete_eq : all_tokens_logits_concrete = prev := extract_eq all_tokens_logits_concrete_value. (*
-Proof. native_cast_no_check (eq_refl prev). Time Qed.*)
+Time Definition all_tokens_logits_concrete_eq : all_tokens_logits_concrete = logits_all_tokens_concrete := extract_eq all_tokens_logits_concrete_value. (*
+Proof. native_cast_no_check (eq_refl logits_all_tokens_concrete). Time Qed.*)
 
-Definition all_tokens_logits : tensor _ _ := PArray.reabstract (fun _ => prea) all_tokens_logits_concrete.
-Lemma all_tokens_logits_eq idxs : all_tokens_logits idxs = prea idxs.
+Definition all_tokens_logits : tensor _ _ := PArray.reabstract (fun _ => logits_all_tokens) all_tokens_logits_concrete.
+Lemma all_tokens_logits_eq idxs : all_tokens_logits idxs = logits_all_tokens idxs.
 Proof.
   cbv [all_tokens_logits].
   erewrite PArray.reabstract_ext_correct by exact all_tokens_logits_concrete_eq.
