theories/TransformerLens/HookedTransformer/Module.v
@@ -467,9 +467,18 @@ End LayerNorm.
 
     | [ |-
         =>
-*)
+ *)
+  (*
+  Set Printing Implicit. Set Printing All.
   Definition logits_all_tokens : tensor _ float
     := HookedTransformer.logits all_tokens.
+  Print logits_all_tokens.
+   *)
+  Notation logits_all_tokens
+    := (@HookedTransformer.logits 1 [Uint63.of_Z (Z.of_N (@pow N N N N_has_pow cfg.d_vocab cfg.n_ctx))] (of_Z (Z.of_N cfg.n_ctx)) float (@coer_refl float) coer_Z_float float_has_add float_has_sub float_has_mul float_has_div float_has_sqrt float_has_exp true (@all_tokens true)).
+
+  Definition logits_all_tokens_concrete : PArray.concrete_tensor _ float
+    := PArray.concretize logits_all_tokens.
 End Model.
 
 Module Type ModelSig (cfg : Config) := Nop <+ Model cfg.
